@prefix : <https://schema.flux.co/> .
@prefix flux: <https://schema.flux.co/> .
@prefix schema: <https://schema.org/> .
@prefix dc: <http://purl.org/dc/terms/> .
@prefix owl: <http://www.w3.org/2002/07/owl#> .
@prefix rdf: <http://www.w3.org/1999/02/22-rdf-syntax-ns#> .
@prefix rdfs: <http://www.w3.org/2000/01/rdf-schema#> .
@prefix xml: <http://www.w3.org/XML/1998/namespace> .
@prefix xsd: <http://www.w3.org/2001/XMLSchema#> .
@base <https://schema.flux.co/> .

<http://schema.flux.co/> a owl:Ontology ;
  owl:versionIRI <http://schema.flux.co/0.1.0/> ;
  owl:imports <https://schema.org> .

#################################################################
#    Classes
#################################################################

flux:SpecifiedQuantity a rdfs:Class ;
  rdfs:subClassOf schema:Intangible .

flux:EthicalConsideration a rdfs:Class ;
  rdfs:subClassOf schema:Intangible ;
  rdfs:comment "Ethical considerations which may affect the consumers purchase"@en ;
  rdfs:label "EthicalConsideration"@en .

flux:AnimalCruelty a rdfs:Class ;
  rdfs:subClassOf flux:EthicalConsideration ;
  rdfs:comment "Defines the known and acknowledged animal cruelty; or the steps taken to ensure there is none"@en ;
  rdfs:label "AnimalCruelty"@en .

flux:ConflictResources a rdfs:Class ;
  rdfs:subClassOf flux:EthicalConsideration ;
  rdfs:comment "Defines the known and acknowledged conflict resources; or the steps taken to ensure there is none"@en ;
  rdfs:label "ConflictResources"@en .

flux:HumanRights a rdfs:Class ;
  rdfs:subClassOf flux:EthicalConsideration ;
  rdfs:comment "Defines the known and acknowledged human rights issues; or the steps taken to ensure there is none"@en ;
  rdfs:label "HumanRights"@en .

flux:LifecycleEmissions a rdfs:Class ;
  rdfs:subClassOf flux:EthicalConsideration ;
  rdfs:comment "Defines the carbon footprint of a product over its lifecycle"@en ;
  rdfs:label "LifecycleEmissions"@en .

flux:Recyclability a rdfs:Class ;
  rdfs:subClassOf flux:EthicalConsideration ;
  rdfs:comment "Gives information on whether and how the product should be recycled by the consumer"@en ;
  rdfs:label "Recyclability"@en .

flux:ProductLifecycleStage a rdfs:Class ;
  rdfs:subClassOf schema:Enumeration ;
  rdfs:comment "Defines part of a product lifecycle"@en ;
  rdfs:label "ProductLifecycleStage"@en .

  ###  Enum Values
  flux:Disposal a flux:ProductLifecycleStage .
  flux:Distribution a flux:ProductLifecycleStage .
  flux:Purchase a flux:ProductLifecycleStage .
  flux:EndOfLife a flux:ProductLifecycleStage .
  flux:Manufacturing a flux:ProductLifecycleStage .
  flux:Usage a flux:ProductLifecycleStage .

flux:FairWagesScheme a rdfs:Class ;
  rdfs:subClassOf schema:Enumeration ;
  rdfs:comment "Defines the schemes an employer might have to ensure fair wages to workers"@en ;
  rdfs:label "FairWagesScheme"@en .

  ###  Enum Values
  flux:MinimumWage a flux:FairWagesScheme ;
    rdfs:comment "The employer is bound by a minimum wage requirement; and pays at least this amount in all the country(s) where work is undertaken"@en ;
    rdfs:label "MinimumWage"@en .
  flux:LivingWage a flux:FairWagesScheme ;
    rdfs:comment "The employer has signed up for relevant 'living wage' schemes in all the country(s) where work is undertaken."@en ;
    rdfs:label "LivingWage"@en .
  flux:TransparentWages a flux:FairWagesScheme ;
    rdfs:comment "The employee wages are transparent (at least to other employees at the same level within the organisation)."@en ;
    rdfs:label "TransparentWages"@en .

#################################################################
#    Annotation properties
#################################################################

flux:ethicalConsideration a rdf:Property ;
  rdfs:comment "Ethical considerations which may affect the consumers purchase"@en ;
  rdfs:label "ethicalConsideration"@en ;
  schema:domainIncludes schema:Product ;
  schema:rangeIncludes flux:EthicalConsideration .

flux:certification a rdf:Property ;
  rdfs:comment "Certification, or certifying body to be used to verify the truthfulness of this statement"@en ;
  rdfs:label "certification"@en ;
  schema:domainIncludes flux:EthicalConsideration ;
  schema:rangeIncludes
    #flux:DigitallySignedCertification,
    schema:URL,
    schema:Text .

flux:productLifecycleStage a rdf:Property ;
  rdfs:comment "Which part(s) of the product lifecycle are affected by this clause"@en ;
  rdfs:label "productLifecycleStage"@en ;
  schema:domainIncludes flux:EthicalConsideration ;
  schema:rangeIncludes flux:ProductLifecycleStage .

flux:emissionsOutput a rdf:Property ;
  rdfs:comment "Assumed estimation of CO2e (or other) resultant emissions"@en ;
  rdfs:label "measuredEmissionsOutput"@en ;
  schema:domainIncludes flux:LifecycleEmissions ;
  schema:rangeIncludes flux:SpecifiedQuantity .

  flux:measuredEmissionsOutput a rdf:Property ;
    rdfs:comment "Measurement of CO2e (or other) resultant emissions"@en ;
    rdfs:label "measuredEmissionsOutput"@en ;
    rdfs:subPropertyOf flux:measuredEmissionsOutput .

  flux:estimatedEmissionsOutput a rdf:Property ;
    rdfs:comment "Estimation of CO2e (or other) resultant emissions"@en ;
    rdfs:label "estimatedEmissionsOutput"@en ;
    rdfs:subPropertyOf flux:measuredEmissionsOutput .

flux:wageFairness a rdf:Property ;
  rdfs:comment "Fairness of pay to the people involved in producing, distributing or selling this product"@en ;
  rdfs:label "wageFairness"@en ;
  schema:domainIncludes flux:HumanRights ;
  schema:rangeIncludes 
    schema:Text,
    flux:FairWagesScheme .

flux:workingConditions a rdf:Property ;
  rdfs:comment "How"@en ;
  rdfs:label "workingConditions"@en ;
  schema:domainIncludes flux:HumanRights ;
  schema:rangeIncludes flux:WorkingConditions .

flux:item a rdf:Property ;
  rdfs:label "item" ;
  rdfs:comment "The represented entity." ;
  schema:domainIncludes flux:SpecifiedQuantity ;
  schema:rangeIncludes
    schema:Text,
    schema:Thing .

flux:quantity a rdf:Property ;
  rdfs:label "quantity" ;
  rdfs:comment "The nominal quantity of the represented entity." ;
  schema:domainIncludes flux:SpecifiedQuantity ;
  schema:rangeIncludes
    schema:Quantity,
    schema:QuantitativeValue .

flux:accuracyBounds a rdf:Property ;
  rdfs:label "accuracyBounds" ;
  rdfs:comment "The amount by which the nominal quantity may be off by in any direction" ;
  schema:domainIncludes flux:SpecifiedQuantity ;
  schema:rangeIncludes
    schema:Quantity,
    schema:QuantitativeValue .

  flux:lowerAccuracyBounds a rdf:Property ;
    rdfs:label "lowerAccuracyBounds" ;
    rdfs:comment "The amount by which the nominal quantity may be off by in the negative direction" ;
    rdfs:subPropertyOf flux:accuracyBounds .

  flux:upperAccuracyBounds a rdf:Property ;
    rdfs:label "upperAccuracyBounds" ;
    rdfs:comment "The amount by which the nominal quantity may be off by in the positive direction" ;
    rdfs:subPropertyOf flux:accuracyBounds .